\makeatletter % Use \makeatletter to make '@' a letter
\def\input@path{{../}} % Define input path to parent directory
\makeatother % Restore default category code of '@'

\documentclass[../main.tex]{subfiles}

\begin{document}

\subsection{Renormalization-scale dependece} \label{subsec:Renormalization_scale_dependence}
In this section we consider renormalization-scale dependence. In principle, such scale $\mu$ should not appear in
the cross sections, as it does not correspond to any fundamental constant or kinematical scale in the problem.
The completely resummed perturbative expansion of an observable is indeed formally independent on $\mu$.
In practise, truncated perturbative expansions exhibit a residual scale dependence, because of neglected higher orders.

We start with deriving the strong coupling $\alpha_s (Q^2)$ as a function of $\alpha_s(\mu^2)$ and $\mu^2/Q^2$, to do so we expand 
the explicit \cref{eq:N4LO} in powers of $\alpha_s(\mu^2)$ and obtain:

\begin{align}
    \begin{split}\label{eq:renormalization scale dependence}
        \alpha_s(Q^2) &= \alpha_s(\mu^2) + \alpha_s^2(\mu^2) b_0 \ln(\frac{\mu^2}{Q^2}) + \alpha_s^3(\mu^2) \biggl[b_1 \ln(\frac{\mu^2}{Q^2}) + b_0^2 \ln^2\qty(\frac{\mu^2}{Q^2})\biggr] \\
        &+ \alpha_s^4 (\mu^2) \biggl[ b_2 \ln(\frac{\mu^2}{Q^2}) + \frac{5}{2} b_0 b_1 \ln^2\qty(\frac{\mu^2}{Q^2}) + b_0^3 \ln^3\qty(\frac{\mu^2}{Q^2})\biggr] \\
        &+ \alpha_s^5(\mu^2) \biggl[ b_3 \ln(\frac{\mu^2}{Q^2}) + \qty(\frac{3}{2} b_1^2 + 3 b_0 b_2 ) \ln^2\qty(\frac{\mu^2}{Q^2}) \\
        &+ \frac{13}{3} b_0^2 b_1 \ln^3\qty(\frac{\mu^2}{Q^2}) + b_0^4 \ln^4\qty(\frac{\mu^2}{Q^2}) \biggr] + \order{\alpha_s^6(\mu^2)}
    \end{split}
\end{align}

for brevity we'll write: 

\begin{equation}
    \alpha_s(Q^2) = \alpha_s(\mu^2) + c_1 \alpha_s^2(\mu^2) + c_2 \alpha_s^3(\mu^2) + c_3 \alpha_s^4(\mu^2) + c_4 \alpha_s^5(\mu^2) + \order{\alpha_s^6(\mu^2)} 
\end{equation}

where $c_i$ are the coefficients of the expansion above.

\begin{align}
    \begin{split}
        c_1 &= b_0 \ln(\frac{\mu^2}{Q^2}) \\
        c_2 &= b_1 \ln(\frac{\mu^2}{Q^2}) + b_0^2 \ln^2\qty(\frac{\mu^2}{Q^2}) \\
        c_3 &= b_2 \ln(\frac{\mu^2}{Q^2}) + \frac{5}{2} b_0 b_1 \ln^2\qty(\frac{\mu^2}{Q^2}) + b_0^3 \ln^3\qty(\frac{\mu^2}{Q^2}) \\
        c_4 &= b_3 \ln(\frac{\mu^2}{Q^2}) + \qty(\frac{3}{2} b_1^2 + 3 b_0 b_2 ) \ln^2\qty(\frac{\mu^2}{Q^2}) + \frac{13}{3} b_0^2 b_1 \ln^3\qty(\frac{\mu^2}{Q^2}) + b_0^4 \ln^4\qty(\frac{\mu^2}{Q^2})
    \end{split}
\end{align}

now we substitute \cref{eq:renormalization scale dependence} into $\lambda = b_0 \alpha_s(Q^2) L$ and obtain: 

\begin{equation}
    \lambda(Q^2) = \lambda(\mu^2) \qty(1 + c_1 \alpha_s(\mu^2) + c_2 \alpha_s^2(\mu^2) + c_3 \alpha_s^3(\mu^2) + c_4 \alpha_s^4(\mu^2) + \order{\alpha_s^5(\mu^2)} )
\end{equation}

and formally expand in powers of $\alpha_s(\mu^2)$ all the relevant functions, now $\lambda = \lambda(\mu^2)$:

\begin{flalign}
    \begin{split}
        L f_1(Q^2) &= L f_1(\lambda) + \frac{c_1}{b_0} \lambda^2 f_1'(\lambda)  + \frac{\lambda}{b_0}\qty(c_2 \lambda f_1'(\lambda) + \frac{1}{2}c_1^2 \lambda^2 f_1''(\lambda)) \textcolor{red}{\alpha_s} \\
        &+ \frac{\lambda}{b_0}\qty(c_3 \lambda f_1'(\lambda) +c_1 c_2 \lambda^2 f_1''(\lambda) +\frac{1}{6}c_1^3 f_1^{(3)}(\lambda) ) \textcolor{blue}{\alpha_s^2} + \frac{\lambda^2}{b_0} \biggl(c_4 f_1'(\lambda) \\
        &+ \frac{1}{2}c_2^2 \lambda f_1''(\lambda) + c_1 c_3 \lambda f_1''(\lambda) +  \frac{1}{2} c_1^2 c_2 \lambda^2 f_1^{(3)}(\lambda) + \frac{1}{24} c_1^4 \lambda^3 f_1^{(4)}(\lambda) \biggr) \textcolor{green}{\alpha_s^3} \\
        f_2(Q^2) &=  f_2(\lambda) + c_1 \lambda f_2'(\lambda) \textcolor{red}{\alpha_s} +\qty(c_2 \lambda f_2'(\lambda) +\frac{1}{2}c_1^2\lambda^2 f_2''(\lambda)) \textcolor{blue}{\alpha_s^2} \\ 
        &+ \qty(c_3 \lambda f_2'(\lambda) + c_1 c_2 \lambda^2 f_2''(\lambda) + \frac{1}{6} c_1^3 f_2^{(3)}(\lambda)) \textcolor{green}{\alpha_s^3} \\
        \textcolor{red}{\alpha_s}f_3(Q^2) &= \textcolor{red}{\alpha_s}f_3(\lambda)  + c_1 \lambda f_3'(\lambda) \textcolor{blue}{\alpha_s^2} + \qty(c_2 \lambda f_3'(\lambda) + \frac{1}{2} c_1^2 \lambda^2 f_3''(\lambda)) \textcolor{green}{\alpha_s^3} \\
        \textcolor{blue}{\alpha_s^2}f_4(Q^2) &= \textcolor{blue}{\alpha_s^2}f_4(\lambda)  + c_1 \lambda f_4'(\lambda) \textcolor{green}{\alpha_s^3} \\
        \textcolor{green}{\alpha_s^3}f_5(Q^2) &= \textcolor{green}{\alpha_s^3}f_5(\lambda) 
    \end{split}
\end{flalign}

As usual, the terms from the expansion proportional to $\textcolor{red}{\alpha_s}$ corrects $f_3$, the terms proportional to $\textcolor{blue}{\alpha_s^2}$ correct $f_4$ and so on. 

So the additional terms in the functions $f_i$ for $i=0,1,3$, to (partially) compensate for the scale change $Q^2\to \mu^2$ therefore read:

\begin{flalign}
    \begin{split}
        \delta f_1\qty(\lambda,\frac{\mu^2}{Q^2}) &= 0 \\
        \delta f_2\qty(\lambda,\frac{\mu^2}{Q^2}) &=  \lambda^2 f_1'(\lambda) \log(\frac{\mu^2}{Q^2}) \\ 
        \delta f_3\qty(\lambda,\frac{\mu^2}{Q^2}) &= \frac{1}{2}\lambda^3 f_1''(\lambda)\log(\frac{\mu^2}{Q^2}) + \lambda^2 f_1'(\lambda) \qty(\log^2\qty(\frac{\mu^2}{Q^2}) + \frac{b1}{b0^2} \log(\frac{\mu^2}{Q^2}))  \\
        &+ \lambda f_2'(\lambda) \log(\frac{\mu^2}{Q^2}) \\
    \end{split}
\end{flalign}

then explicitly calculate those derivatives and obtain the scale dependence.

\end{document}